@prefix : <https://w3id.org/stax/ontology#> .
@prefix dc: <http://purl.org/dc/elements/1.1/> .
@prefix owl: <http://www.w3.org/2002/07/owl#> .
@prefix rdf: <http://www.w3.org/1999/02/22-rdf-syntax-ns#> .
@prefix xml: <http://www.w3.org/XML/1998/namespace> .
@prefix xsd: <http://www.w3.org/2001/XMLSchema#> .
@prefix foaf: <http://xmlns.com/foaf/0.1/> .
@prefix rdfs: <http://www.w3.org/2000/01/rdf-schema#> .
@prefix skos: <http://www.w3.org/2004/02/skos/core#> .
@prefix stax: <https://w3id.org/stax/ontology#> .
@prefix vann: <http://purl.org/vocab/vann/> .
@prefix schema: <http://schema.org/> .
@prefix dcterms: <http://purl.org/dc/terms/> .
@prefix stax_ont: <https://w3id.org/stax/ontology> .
@base <https://w3id.org/stax/ontology> .

<https://w3id.org/stax/ontology> rdf:type owl:Ontology ;
                                  owl:imports <http://www.w3.org/TR/skos-reference/skos-owl1-dl.rdf> ;
                                  dc:description "RDF-STaX is an OWL 2 DL ontology that enables describing the types of RDF streams and defines relations between them."@en ;
                                  dc:title "RDF Stream Taxonomy (RDF-STaX)"@en ;
                                  dcterms:created "2023-10-22T00:00:00"^^xsd:dateTime ;
                                  dcterms:issued "2023-10-23T00:00:00"^^xsd:dateTime ;
                                  dcterms:license <https://spdx.org/licenses/CC-BY-4.0> ;
                                  vann:preferredNamespacePrefix "stax" ;
                                  vann:preferredNamespaceUri stax: ;
                                  schema:citation "Please cite this ontology according to the instructions here: https://w3id.org/stax/dev/licensing/"@en ;
                                  skos:altLabel "RDF-STaX"@en ;
                                  skos:prefLabel "RDF Stream Taxonomy"@en ;
                                  foaf:homepage <https://w3id.org/stax> .

#################################################################
#    Annotation properties
#################################################################

###  http://purl.org/dc/elements/1.1/description
dc:description rdf:type owl:AnnotationProperty .


###  http://purl.org/dc/elements/1.1/title
dc:title rdf:type owl:AnnotationProperty .


###  http://purl.org/dc/terms/created
dcterms:created rdf:type owl:AnnotationProperty .


###  http://purl.org/dc/terms/issued
dcterms:issued rdf:type owl:AnnotationProperty .


###  http://purl.org/dc/terms/license
dcterms:license rdf:type owl:AnnotationProperty .


###  http://purl.org/vocab/vann/preferredNamespacePrefix
vann:preferredNamespacePrefix rdf:type owl:AnnotationProperty .


###  http://purl.org/vocab/vann/preferredNamespaceUri
vann:preferredNamespaceUri rdf:type owl:AnnotationProperty .


###  http://schema.org/citation
schema:citation rdf:type owl:AnnotationProperty .


###  http://xmlns.com/foaf/0.1/homepage
foaf:homepage rdf:type owl:AnnotationProperty .


#################################################################
#    Object Properties
#################################################################

###  https://w3id.org/stax/ontology#canBeFlattenedInto
stax:canBeFlattenedInto rdf:type owl:ObjectProperty ;
                        rdfs:subPropertyOf stax:streamTypeSemanticRelation ;
                        owl:propertyChainAxiom ( skos:broaderTransitive
                                                 stax:canBeFlattenedInto
                                               ) ;
                        rdfs:comment """Indicates that the subject stream type can be flattened into the object.

The flattening is done by enumerating all components of the stream elements in one, flat stream. For example, a graph stream can be flattened into a flat triple stream."""@en ;
                        rdfs:label "can be flattened into"@en .


###  https://w3id.org/stax/ontology#canBeGroupedInto
stax:canBeGroupedInto rdf:type owl:ObjectProperty ;
                      rdfs:subPropertyOf stax:streamTypeSemanticRelation ;
                      owl:propertyChainAxiom ( skos:broaderTransitive
                                               stax:canBeGroupedInto
                                             ) ;
                      rdfs:comment """Indicates that the subject stream type can be grouped into the object.

The grouping is done by splitting the flat stream of statements into groups, which then can be used to construct elements of the grouped stream. For example, a flat triple stream can be grouped into a graph stream. In this operation, the ordering information within a group is lost."""@en ;
                      rdfs:label "can be grouped into"@en .


###  https://w3id.org/stax/ontology#canBeTriviallyExtendedInto
stax:canBeTriviallyExtendedInto rdf:type owl:ObjectProperty ;
                                rdfs:subPropertyOf stax:streamTypeSemanticRelation ;
                                owl:propertyChainAxiom ( skos:broaderTransitive
                                                         stax:canBeTriviallyExtendedInto
                                                       ) ;
                                rdfs:comment """Indicates that the subject stream type that uses triples or graphs can be trivially extended into the object type that uses quads or datasets.

The extension is done by (in case of flat RDF streams) adding a fourth component, corresponding to the default graph. In case of grouped RDF streams, the contents of the graph are placed explicitly in the default graph."""@en ;
                                rdfs:label "can be trivially extended into"@en .


###  https://w3id.org/stax/ontology#hasElementType
stax:hasElementType rdf:type owl:ObjectProperty ;
                    rdfs:domain stax:ConcreteRdfStreamType ;
                    rdfs:range stax:RdfElementType ;
                    owl:propertyChainAxiom ( skos:broaderTransitive
                                             stax:hasElementType
                                           ) ;
                    rdfs:comment "For an RDF stream type, indicates the base (primitive) type of elements in the stream (e.g., triple, quad, graph, dataset)."@en ;
                    rdfs:label "has element type"@en .


###  https://w3id.org/stax/ontology#hasStreamType
stax:hasStreamType rdf:type owl:ObjectProperty ;
                   rdfs:domain stax:RdfStreamTypeUsage ;
                   rdfs:range stax:ConcreteRdfStreamType ;
                   rdfs:comment "For an RDF stream type usage, this property indicates which stream type is used."@en ;
                   rdfs:label "has stream type"@en .


###  https://w3id.org/stax/ontology#hasStreamTypeUsage
stax:hasStreamTypeUsage rdf:type owl:ObjectProperty ;
                        owl:inverseOf stax:isUsageOf ;
                        rdfs:range stax:RdfStreamTypeUsage ;
                        rdfs:comment """Inverse of stax:isUsageOf – indicates that the subject is related to a usage of an RDF stream type.

The subject for this property can be for example a published stream on the Web (e.g., vocals:RDFStream) or a scientific publication that discusses a usage of an RDF stream type."""@en ;
                        rdfs:label "has stream type usage"@en .


###  https://w3id.org/stax/ontology#isUsageOf
stax:isUsageOf rdf:type owl:ObjectProperty ;
               rdfs:domain stax:RdfStreamTypeUsage ;
               rdfs:comment """For an RDF stream type usage, this property indicates where the stream was used or from where the usage was derived. The value of this property can be anything that makes sense for the desired use case. The value can be for example: the DOI URL of an academic work, URL of a piece of software, IRI of a published stream, IRI of an RDF dataset.

Inverse of stax:hasStreamTypeUsage."""@en ;
               rdfs:label "is usage of"@en .


###  https://w3id.org/stax/ontology#streamTypeSemanticRelation
stax:streamTypeSemanticRelation rdf:type owl:ObjectProperty ;
                                rdfs:subPropertyOf skos:semanticRelation ;
                                rdfs:domain stax:ConcreteRdfStreamType ;
                                rdfs:range stax:ConcreteRdfStreamType ;
                                rdfs:comment "This property should not be used directly, but as a super-property for all properties denoting a relationship of meaning between RDF stream types."@en ;
                                rdfs:label "is in stream type semantic relation with"@en .


#################################################################
#    Classes
#################################################################

###  https://w3id.org/stax/ontology#AbstractRdfStreamType
stax:AbstractRdfStreamType rdf:type owl:Class ;
                           rdfs:subClassOf stax:RdfStreamType ;
                           owl:disjointWith stax:ConcreteRdfStreamType ;
                           rdfs:comment "Class for abstract RDF stream types in the taxonomy. Instances of this class have abstract definitions, i.e., they cannot be used to annotate real streams. They are only intended to be used for reasoning about stream types."@en ;
                           rdfs:label "Abstract RDF stream type"@en .


###  https://w3id.org/stax/ontology#ConcreteRdfStreamType
stax:ConcreteRdfStreamType rdf:type owl:Class ;
                           rdfs:subClassOf stax:RdfStreamType ,
                                           [ rdf:type owl:Restriction ;
                                             owl:onProperty stax:hasElementType ;
                                             owl:someValuesFrom stax:RdfElementType
                                           ] ,
                                           [ rdf:type owl:Restriction ;
                                             owl:onProperty stax:hasElementType ;
                                             owl:allValuesFrom stax:RdfElementType
                                           ] ;
                           rdfs:comment "Class for the concrete RDF stream types in the taxonomy. Instances of this class have concrete definitions, and they can be used to annotate real streams."@en ;
                           rdfs:label "Concrete RDF stream type"@en .


###  https://w3id.org/stax/ontology#RdfElementType
stax:RdfElementType rdf:type owl:Class ;
                    owl:equivalentClass [ rdf:type owl:Class ;
                                          owl:oneOf ( stax:dataset
                                                      stax:graph
                                                      stax:quad
                                                      stax:triple
                                                    )
                                        ] ;
                    owl:disjointWith stax:RdfStreamType ;
                    rdfs:comment "Class for base types of elements in RDF streams. There are four instances of this class (triple, quad, graph, dataset) and they should not be further specialized. The instances of this class do NOT form a taxonomical structure."@en ;
                    rdfs:label "RDF element type"@en .


###  https://w3id.org/stax/ontology#RdfStreamType
stax:RdfStreamType rdf:type owl:Class ;
                   rdfs:subClassOf skos:Concept ;
                   rdfs:comment "Base class for RDF stream types. This class should not be used directly – use instead either stax:AbstractRdfStreamType or stax:ConcreteRdfStreamType."@en ;
                   rdfs:label "RDF stream type"@en .


###  https://w3id.org/stax/ontology#RdfStreamTypeUsage
stax:RdfStreamTypeUsage rdf:type owl:Class ;
                        rdfs:subClassOf [ rdf:type owl:Restriction ;
                                          owl:onProperty stax:hasStreamType ;
                                          owl:allValuesFrom stax:ConcreteRdfStreamType
                                        ] ;
                        rdfs:comment """Class for instances of using an RDF stream type, in a program, an academic paper, or elsewhere. This class is suitable for annotating both theoretical uses and practical ones, i.e., real streams or datasets.

Instances of this class should have the stax:hasStreamType property pointing to a concrete stream type. The stax:usedIn property is recommended to indicate where the stream is used – alternatively you can use its inverse (stax:hasStreamTypeUsage). The use of other properties (e.g., rdfs:label, rdfs:comment) is encouraged to give more context about the usage.

Note that \"stream type usage\" is a subjective assertion and instances of this class may be annotated with additional provenance properties to explain who made the assertion. There can be multiple views on what type of stream is in use, depending on the involved actor, processing step, etc."""@en ;
                        rdfs:label "RDF stream type usage"@en ;
                        skos:example <https://w3id.org/stax/dev/use-it/> .


#################################################################
#    Individuals
#################################################################

###  https://w3id.org/stax/ontology
<https://w3id.org/stax/ontology> rdf:type owl:NamedIndividual ,
                                          skos:ConceptScheme ;
                                 skos:hasTopConcept stax:rdfStream .


###  https://w3id.org/stax/ontology#dataset
stax:dataset rdf:type owl:NamedIndividual ,
                      stax:RdfElementType ;
             skos:definition <https://www.w3.org/TR/rdf11-concepts/#section-dataset> ;
             skos:note "RDF dataset, as defined by the RDF 1.1 Concepts and Abstract Syntax W3C Recommendation."@en ;
             skos:prefLabel "RDF dataset"@en .


###  https://w3id.org/stax/ontology#datasetStream
stax:datasetStream rdf:type owl:NamedIndividual ,
                            stax:ConcreteRdfStreamType ;
                   skos:broader stax:groupedStream ;
                   skos:inScheme <https://w3id.org/stax/ontology> ;
                   stax:canBeFlattenedInto stax:flatQuadStream ;
                   stax:hasElementType stax:dataset ;
                   skos:definition "An RDF dataset stream is a grouped RDF stream whose elements are RDF datasets."@en ;
                   skos:example <https://w3id.org/np/RAcku4ZQ6KWKFF2uLthK3mqCCNfWbrEeN643SVXwjXseE> ,
                                <https://w3id.org/np/RAq7ctp_pHq3u76I54CU9S4WA4L9wQFCnmj3DJyrfrL58> ;
                   skos:note "A stream of RDF datasets."@en ;
                   skos:prefLabel "RDF dataset stream"@en .


###  https://w3id.org/stax/ontology#flatQuadStream
stax:flatQuadStream rdf:type owl:NamedIndividual ,
                             stax:ConcreteRdfStreamType ;
                    skos:broader stax:flatStream ;
                    skos:inScheme <https://w3id.org/stax/ontology> ;
                    stax:canBeGroupedInto stax:datasetStream ;
                    stax:hasElementType stax:quad ;
                    skos:definition "A flat RDF quad stream is a flat RDF stream whose elements are quad statements."@en ;
                    skos:example <https://w3id.org/np/RAZIs-6LyJuxrn-osVbEdxEoXmGsC1g-8m3n8LYAZ6sUI> ;
                    skos:note "A stream of quad statements."@en ;
                    skos:prefLabel "Flat RDF quad stream"@en .


###  https://w3id.org/stax/ontology#flatStream
stax:flatStream rdf:type owl:NamedIndividual ,
                         stax:AbstractRdfStreamType ;
                skos:broader stax:rdfStream ;
                skos:inScheme <https://w3id.org/stax/ontology> ;
                skos:definition "A flat RDF stream is an RDF stream whose elements are statements (either RDF triples or RDF quads)."@en ;
                skos:note "Abstract flat RDF stream type."@en ;
                skos:prefLabel "Flat RDF stream"@en .


###  https://w3id.org/stax/ontology#flatTripleStream
stax:flatTripleStream rdf:type owl:NamedIndividual ,
                               stax:ConcreteRdfStreamType ;
                      skos:broader stax:flatStream ;
                      skos:inScheme <https://w3id.org/stax/ontology> ;
                      stax:canBeGroupedInto stax:graphStream ;
                      stax:canBeTriviallyExtendedInto stax:flatQuadStream ;
                      stax:hasElementType stax:triple ;
                      skos:definition "A flat RDF triple stream is a flat RDF stream whose elements are triple statements."@en ;
                      skos:example <https://w3id.org/np/RAelRRiQeq2oSXNR-qqrB5dQ6g7Lait55srza_sfz6Jzs> ,
                                   <https://w3id.org/np/RAsiMOcZpJwtQVyiIBvn5-K1AvCcXmU8axm9VY4A7AY-k> ;
                      skos:note "A stream of triple statements."@en ;
                      skos:prefLabel "Flat RDF triple stream"@en .


###  https://w3id.org/stax/ontology#graph
stax:graph rdf:type owl:NamedIndividual ,
                    stax:RdfElementType ;
           skos:definition <https://www.w3.org/TR/rdf11-concepts/#section-rdf-graph> ;
           skos:note "RDF graph, as defined by the RDF 1.1 Concepts and Abstract Syntax W3C Recommendation."@en ;
           skos:prefLabel "RDF graph"@en .


###  https://w3id.org/stax/ontology#graphStream
stax:graphStream rdf:type owl:NamedIndividual ,
                          stax:ConcreteRdfStreamType ;
                 skos:broader stax:groupedStream ;
                 skos:inScheme <https://w3id.org/stax/ontology> ;
                 stax:canBeFlattenedInto stax:flatTripleStream ;
                 stax:canBeTriviallyExtendedInto stax:datasetStream ;
                 stax:hasElementType stax:graph ;
                 skos:definition "An RDF graph stream is a grouped RDF stream whose elements are unnamed (default) RDF graphs."@en ;
                 skos:example <https://w3id.org/np/RA2LEhdLOYY_c9YgGIwu9TrzHVFPQcpE2vMnAbPghQY60> ,
                              <https://w3id.org/np/RA9jYlusATe999AN0jb6fn4eR_H4Q23xhnwU4xSwuUxQw> ;
                 skos:note "A stream of RDF graphs."@en ;
                 skos:prefLabel "RDF graph stream"@en .


###  https://w3id.org/stax/ontology#groupedStream
stax:groupedStream rdf:type owl:NamedIndividual ,
                            stax:AbstractRdfStreamType ;
                   skos:broader stax:rdfStream ;
                   skos:inScheme <https://w3id.org/stax/ontology> ;
                   skos:definition "A grouped RDF stream is an RDF stream whose elements are either RDF graphs or RDF datasets."@en ;
                   skos:note "Abstract grouped RDF stream type."@en ;
                   skos:prefLabel "Grouped RDF stream"@en .


###  https://w3id.org/stax/ontology#namedGraphStream
stax:namedGraphStream rdf:type owl:NamedIndividual ,
                               stax:ConcreteRdfStreamType ;
                      skos:broader stax:datasetStream ;
                      skos:inScheme <https://w3id.org/stax/ontology> ;
                      skos:definition "An RDF named graph stream is an RDF dataset stream in which every element has exactly one named RDF graph pair <n, G>, where G is an RDF graph, and n is the graph node. Apart from graph G, the dataset may contain any number of triples in the default graph."@en ;
                      skos:example <https://w3id.org/np/RAxK3wEoSabXMV2_s24gd27O8rzsUFceYeMKn5s04cnkk> ;
                      skos:note "A stream of datasets which have one named graph."@en ;
                      skos:prefLabel "RDF named graph stream"@en .


###  https://w3id.org/stax/ontology#quad
stax:quad rdf:type owl:NamedIndividual ,
                   stax:RdfElementType ;
          skos:definition "An RDF quad is an RDF triple with a fourth component indicating the RDF graph the triple belongs to. If the triple is in a named graph, then the fourth component is the graph name (blank node or IRI). If the triple is in the default graph, then the fourth component is empty."@en ;
          skos:note "RDF quad, defined here in STaX. The definition is based on the RDF 1.1 Concepts and Abstract Syntax W3C Recommendation."@en ;
          skos:prefLabel "RDF quad"@en .


###  https://w3id.org/stax/ontology#rdfStream
stax:rdfStream rdf:type owl:NamedIndividual ,
                        stax:AbstractRdfStreamType ;
               skos:topConceptOf <https://w3id.org/stax/ontology> ;
               skos:definition "An RDF stream is an ordered, potentially infinite sequence of RDF stream elements."@en ;
               skos:note "Base abstract RDF stream type."@en ;
               skos:prefLabel "RDF stream"@en .


###  https://w3id.org/stax/ontology#subjectGraphStream
stax:subjectGraphStream rdf:type owl:NamedIndividual ,
                                 stax:ConcreteRdfStreamType ;
                        skos:broader stax:graphStream ;
                        skos:inScheme <https://w3id.org/stax/ontology> ;
                        skos:definition "An RDF subject graph stream is an RDF graph stream in which every element contains an IRI node (called the subject node) that uniquely identifies the graph in the stream. Every other node in the graph can be reached by traversing triples, starting from the subject node."@en ;
                        skos:example <https://w3id.org/np/RAD3_KmaQcSOOQTOKOsrwahi56Ib8pKMRlKfhylozW-UQ> ,
                                     <https://w3id.org/np/RAqbZ03A1F0UPJmpa6d_r_uRUp46nmcwN8Yep2Rgiy8b4> ;
                        skos:note "A stream of RDF graphs which have a node that uniquely identifies them in the stream."@en ;
                        skos:prefLabel "RDF subject graph stream"@en .


###  https://w3id.org/stax/ontology#timestampedNamedGraphStream
stax:timestampedNamedGraphStream rdf:type owl:NamedIndividual ,
                                          stax:ConcreteRdfStreamType ;
                                 skos:broader stax:namedGraphStream ;
                                 skos:inScheme <https://w3id.org/stax/ontology> ;
                                 skos:definition """A timestamped named graph is an RDF dataset in which: (1) there is exactly one named RDF graph pair <n, G>, where G is an RDF graph, and n is the graph node; (2) the default graph includes a timestamp triple <n, p, t>, where p is a timestamp predicate that relates t, called the timestamp, and the graph G.

A timestamped RDF named graph stream is an RDF named graph stream in which every element is a timestamped named graph. The elements that share the same timestamp predicate p are ordered by the partial order associated with p."""@en ;
                                 skos:example <https://w3id.org/np/RA6E9BH7J5qMYnuL7Kgys4Vsz25AKIAHtSQ78tcXFIlTc> ,
                                              <https://w3id.org/np/RAU7pbHsOVgltc5Az1pOuNSV4cjI-DDWqoRJyAVhKvUus> ;
                                 skos:note "A stream of datasets which contain one timestamped, named graph. The definition is based on the draft RSP Data model: https://streamreasoning.org/RSP-QL/Abstract%20Syntax%20and%20Semantics%20Document/"@en ;
                                 skos:prefLabel "Timestamped RDF named graph stream"@en .


###  https://w3id.org/stax/ontology#triple
stax:triple rdf:type owl:NamedIndividual ,
                     stax:RdfElementType ;
            skos:definition <https://www.w3.org/TR/rdf11-concepts/#section-triples> ;
            skos:note "RDF triple, as defined by the RDF 1.1 Concepts and Abstract Syntax W3C Recommendation."@en ;
            skos:prefLabel "RDF triple"@en .


###  Generated by the OWL API (version 4.5.9.2019-02-01T07:24:44Z) https://github.com/owlcs/owlapi
